Complicate the whole matter. Slightly more than I wanted.

thy/AbstractInterpretation.thy
@@ -10,6 +10,24 @@ fun destrmi :: "nat \<Rightarrow> bdd \<Rightarrow> (nat, nat) IFEXD" where
 "destrmi (Suc 0) bdd = TD" |
 "destrmi (Suc (Suc n)) bdd = (case pm_pth bdd n of (v, t, e) \<Rightarrow> IFD v t e)"
 
+definition "bdd_node_valid bdd n \<equiv> n < 2 \<or> pointermap_p_valid (n - 2) bdd"
+lemma [simp]: 
+  "bdd_node_valid bdd 0"
+  "bdd_node_valid bdd (Suc 0)"
+  by (auto simp: bdd_node_valid_def)
+  
+definition "ifexd_valid bdd e \<equiv> (case e of IFD _ t e \<Rightarrow> bdd_node_valid bdd t \<and> bdd_node_valid bdd e | _ \<Rightarrow> True)"
+definition "bdd_sane bdd \<equiv> pointermap_sane bdd \<and> (\<forall>n. bdd_node_valid bdd n \<longrightarrow> ifexd_valid bdd (destrmi n bdd))"
+
+lemma ifexd_validI: 
+	assumes sane: "bdd_sane bdd" and valid: "bdd_node_valid bdd n"
+	shows "ifexd_valid bdd (destrmi n bdd)" 
+proof(cases "destrmi n bdd")
+	case (IFD v t e)
+	note mp[OF spec[OF conjunct2[OF sane[unfolded bdd_sane_def]]], OF valid]
+	thus ?thesis .
+qed(simp_all add: ifexd_valid_def)
+
 fun tmi where "tmi bdd = (1, bdd)"
 fun fmi where "fmi bdd = (0, bdd)"
 fun ifmi :: "nat \<Rightarrow> nat \<Rightarrow> nat \<Rightarrow> bdd \<Rightarrow> (nat \<times> bdd)" where
@@ -22,6 +40,13 @@ fun Rmi_g :: "nat \<Rightarrow> nat ifex \<Rightarrow> bdd \<Rightarrow> bool" w
 "Rmi_g _ _ _ = False"
 
 definition "Rmi s \<equiv> {(a,b)|a b. Rmi_g a b s}"
+
+
+lemma bdd_node_valid_RmiI: "(ni,n)\<in>Rmi bdd \<Longrightarrow> bdd_node_valid bdd ni"
+  apply (auto simp: Rmi_def)
+  apply (cases "(ni,n,bdd)" rule: Rmi_g.cases; simp)
+  apply (auto simp: bdd_node_valid_def)
+  done
 
 lemma prod_split3: "P (case prod of (x, xa, xaa) \<Rightarrow> f x xa xaa) = (\<forall>x1 x2 x3. prod = (x1, x2, x3) \<longrightarrow> P (f x1 x2 x3))"
 by(simp split: prod.splits)
@@ -128,20 +153,224 @@ lemma in_lesI:
     shows "(ni1, n1) \<in> Rmi s'" "(ni2, n2) \<in> Rmi s'"
 by (meson assms bdd_impl_pre.les_def)+
 
-interpretation brofix!: bdd_impl_eq pointermap_sane Rmi tmi fmi ifmi destrmi
+(*lemma nat_minus2ne_hlp: "\<lbrakk>2 \<le> n; n \<noteq> ni\<rbrakk> \<Longrightarrow> ni - 2 \<noteq> (n :: nat) - 2" 
+proof(cases "2 \<le> ni")
+	case True
+	then obtain ni' where[simp]: "ni = Suc (Suc ni')" using add_2_eq_Suc le_Suc_ex by blast
+	assume "2 \<le> n"
+	then obtain n' where[simp]: "n = Suc (Suc n')" using add_2_eq_Suc le_Suc_ex by blast
+	assume "n \<noteq> ni"
+	thus ?thesis by simp
+next
+	assume "2 \<le> n"
+	moreover case False
+	ultimately show ?thesis nitpick 
+qed simp
+sorry*)
+
+(*lemma le2ne_hlp: " \<lbrakk>\<not> n < 2; Suc (Suc n) \<noteq> Suc (Suc ni)\<rbrakk> \<Longrightarrow> ni - 2 \<noteq> n - 2" nitpick oops
+lemma le2ne_hlp: 
+	fixes ni x :: nat
+	assumes ne: "ni \<noteq> n" 
+	assumes gni: "2 \<le> ni" and gn: " 2 \<le> n"
+	shows "ni - 2 \<noteq> n - 2" using assms by simp
+proof -
+	from gni obtain ni' where[simp]: "ni = Suc (Suc ni')" using add_2_eq_Suc le_Suc_ex by blast
+	from gn obtain n' where[simp]: "n = Suc (Suc n')" using add_2_eq_Suc le_Suc_ex by blast
+	show ?thesis using ne by simp
+qed*)
+
+lemma ifmi_valid_set_modification:
+	assumes ifm: "ifmi v ni1 ni2 s = (ni, s')"
+	assumes ne: "ni1 \<noteq> ni2"
+	shows "{n. bdd_node_valid s' n} \<subseteq> insert ni {n. bdd_node_valid s n}"
+proof
+	case goal1
+	hence bv: "bdd_node_valid s' x" by simp
+	thus ?case proof(cases "x = ni")
+		case True thus ?thesis by simp
+	next
+		case False thus ?thesis proof(cases "x < 2")
+			case True thus ?thesis by(simp add: bdd_node_valid_def)
+		next
+			case False
+			have gni: "2 \<le> ni" using ifm ne by(simp add: apfst_def map_prod_def split: prod.splits)
+			have pv: "pointermap_p_valid (x - 2) s'" using bv False unfolding bdd_node_valid_def by simp
+			have ne': "ni - 2 \<noteq> x - 2" using `x \<noteq> ni` gni False by simp
+			have "pointermap_p_valid (x - 2) s" using ifm ne' 
+				by(auto simp add: ne apfst_def map_prod_def split: prod.splits dest: pointermap_backward_valid[OF pv])
+			thus ?thesis by(simp add: bdd_node_valid_def)
+		qed
+	qed
+qed
+(*next
+	case goal2 show ?case proof
+		case goal1 thus ?case proof(cases "x = ni")
+			case True thus ?thesis using ifm ne apply(clarsimp simp add: apfst_def map_prod_def bdd_node_valid_def split: prod.splits) apply(rule pointermap_sane_getmkD)*)
+
+lemma ifmi_saneI2:
+	assumes sane: "bdd_sane s"
+	assumes valid: "bdd_node_valid s ni1"  "bdd_node_valid s ni2" 
+	assumes ifm: "ifmi v ni1 ni2 s = (ni, s')"
+	shows "bdd_sane s'"
+proof -
+	have pms: "pointermap_sane s" using sane[unfolded bdd_sane_def] by simp
+	hence pms': "pointermap_sane s'" using ifm ifmi_saneI by blast
+	moreover { 
+		fix n 
+		assume sv: "bdd_node_valid s' n"
+		have "ifexd_valid s' (destrmi n s') \<Longrightarrow> True" 
+		(*proof(cases "n < 2")
+			case True thus ?thesis by(simp add: ifexd_valid_def)
+		proof(cases "n = ni ")
+			case True
+			thus ?thesis using ifm unfolding True
+				apply(simp split: if_splits) 
+				apply(rule ifexd_validI)
+				using sane apply(simp;fail)
+				using sv apply(simp;fail)
+				apply(simp add: comp_def apfst_def map_prod_def  split: prod.splits)
+				apply(cases "(ni, s')" rule: destrmi.cases)
+				apply(simp_all)
+				apply(frule pointermap_update_pthI[OF pms])
+				apply(simp add: ifexd_valid_def)
+				apply(simp add: bdd_node_valid_def)
+				apply(rule)
+				using valid(1) apply(cases "ni1 < 2"; simp add: bdd_node_valid_def pointermap_p_valid_inv; fail)
+				using valid(2) apply(cases "ni2 < 2"; simp add: bdd_node_valid_def pointermap_p_valid_inv; fail)
+			done
+		next
+			case False
+			thus ?thesis proof(cases "(n, s')" rule: destrmi.cases)
+				case (3 nx bdd) 
+				note s' = 3[unfolded prod.simps]
+				note s = conjunct1[OF s'] conjunct2[OF s']
+				have "bdd_node_valid s n" 
+					apply(cases "ni1 = ni2")
+					 using ifm sv apply(simp)
+					using sv unfolding bdd_node_valid_def apply(cases "n < 2") apply(simp_all) 
+					apply(rule pointermap_backward_valid[of _ _ _ _ "ni - 2"])
+					  apply(assumption) 
+					 using ifm apply(auto simp: apfst_def map_prod_def comp_def split: prod.splits)[1]
+					using False apply - apply(rule ccontr, unfold not_not)
+				done
+				thus ?thesis 
+				
+				sorry
+			qed (simp_all add: ifexd_valid_def)
+				(* 
+				note ifm[unfolded ifmi.simps apfst_def map_prod_def comp_def]
+				hence "ni1 \<noteq> ni2 \<Longrightarrow> pointermap_getmk (v, ni1, ni2) s = (ni - 2, s')"
+			apply(simp split: prod.splits) sorry
+			have "bdd_node_valid s n" 
+				apply(cases "ni1 = ni2")
+				 using ifm sv apply(simp)
+				using sv unfolding bdd_node_valid_def apply(cases "n < 2") apply(simp_all) 
+				apply(rule pointermap_backward_valid[of _ _ _ _ "ni - 2"])
+				  apply(assumption) 
+				 using ifm apply(auto simp: apfst_def map_prod_def comp_def split: prod.splits)[1]
+			done
+			note mp[OF spec[OF conjunct2[OF sane[unfolded bdd_sane_def]]], OF this]*)
+				using ifm
+				apply(cases "(n, s')" rule: destrmi.cases)
+				apply(simp add: ifexd_valid_def;fail)+
+				apply(simp del: ifmi.simps split: prod.splits)
+				using pointermap_p_pth_inv[OF pv]
+				apply -
+				apply(simp split: if_splits) 
+				apply(rule ifexd_validI)
+				using sane apply(simp;fail)
+				using sv apply(simp;fail)
+				apply(cases "(n, s')" rule: destrmi.cases)
+				apply(simp add: ifexd_valid_def;fail)+
+				apply(simp add: comp_def apfst_def map_prod_def split: prod.splits)
+				using sv
+				apply(clarsimp)
+				apply(frule pointermap_backward_valid[OF pv])
+				apply force
+				apply(clarsimp)
+				apply(frule (1) pointermap_p_pth_inv[of _ s])
+				apply(simp)
+				using mp[OF spec[OF conjunct2[OF sane[unfolded bdd_sane_def]]]]
+				apply(rule)
+				find_theorems "pointermap_getmk"
+				apply(rule)
+				apply(simp add: pms')
+				apply(simp add: comp_def apfst_def map_prod_def  split: prod.splits)
+				
+				
+			sorry
+		qed*) sorry
+	}
+	have vp: "\<forall>n. bdd_node_valid s n \<longrightarrow> ifexd_valid s (destrmi n s)" using sane unfolding bdd_sane_def by simp
+	have "(\<forall>n. bdd_node_valid s' n \<longrightarrow> ifexd_valid s' (destrmi n s'))"
+	proof(cases "ni1 = ni2")
+		case True thus ?thesis using vp ifm by simp
+	next
+		case False
+		have "\<forall>n. (n = ni \<or> bdd_node_valid s n) \<longrightarrow> ifexd_valid s' (destrmi n s')"
+		proof(clarify)
+			fix n
+			assume eov: "n = ni \<or> bdd_node_valid s n"
+			have gmk: "pointermap_getmk (v, ni1, ni2) s = (ni - 2, s')"
+				using ifm by(clarsimp simp: `ni1 \<noteq> ni2` apfst_def map_prod_def split: prod.splits)
+			hence dme: "destrmi ni s' = IFD v ni1 ni2"
+				using ifm pointermap_update_pthI[OF pms gmk]
+				by(cases "(ni, s')" rule: destrmi.cases)
+				  (clarsimp simp: `ni1 \<noteq> ni2` apfst_def map_prod_def pointermap_update_pthI[OF pms gmk] split: prod.splits)+
+			show "ifexd_valid s' (destrmi n s')"
+			proof(cases "n = ni")
+				case True
+					show "ifexd_valid s' (destrmi n s')" unfolding True
+					using ifm
+					apply(clarsimp simp: False apfst_def map_prod_def split: prod.splits)
+					apply(clarsimp simp: ifexd_valid_def)
+					apply(frule pointermap_update_pthI[OF pms])
+					apply(rename_tac a b)
+					apply(rule)
+					using valid(1) apply(case_tac "a < 2"; simp add: bdd_node_valid_def pointermap_p_valid_inv; fail)
+					using valid(2) apply(case_tac "b < 2"; simp add: bdd_node_valid_def pointermap_p_valid_inv)
+				done
+			next
+				case False
+				with eov have nv: "bdd_node_valid s n" by simp
+				with vp have dv: "ifexd_valid s (destrmi n s)" by simp
+				thus ?thesis proof(cases "(n, s')" rule: destrmi.cases)
+					case (3 p bdd)
+					with nv have pv: "pointermap_p_valid p s" unfolding bdd_node_valid_def by auto
+					note ifm[unfolded ifmi.simps if_not_P[OF `ni1 \<noteq> ni2`] apfst_def map_prod_def comp_def id_def]
+					show ?thesis 
+						using dv 3 pointermap_p_pth_inv[OF pv gmk] gmk
+						apply(clarsimp split: prod.splits)
+						apply(clarsimp simp: ifexd_valid_def)
+						apply(rename_tac a b)
+						apply(rule)
+						apply(case_tac "a < 2"; simp add: bdd_node_valid_def pointermap_p_valid_inv; fail)
+						apply(case_tac "b < 2"; simp add: bdd_node_valid_def pointermap_p_valid_inv; fail)
+					done
+				qed (simp_all add: ifexd_valid_def)
+			qed
+		qed
+		with ifmi_valid_set_modification[OF ifm False]
+		show ?thesis by blast
+	qed
+	with pms' show ?thesis unfolding bdd_sane_def by blast
+qed
+
+interpretation brofix!: bdd_impl_eq bdd_sane Rmi tmi fmi ifmi destrmi
 proof  -
   note s = bdd_impl_pre.les_def[simp] Rmi_def[simp]
-	show "bdd_impl_eq pointermap_sane Rmi tmi fmi ifmi destrmi"
+	show "bdd_impl_eq bdd_sane Rmi tmi fmi ifmi destrmi"
 	proof(unfold_locales)
 	     case goal1 thus ?case by(clarsimp split: if_splits)
 	next case goal2 thus ?case by(clarsimp split: if_splits)
-	next case goal3 thus ?case using ifmi_les by blast
+	next case goal3 thus ?case using ifmi_les bdd_sane_def by blast
 	next case goal4 thus ?case by(clarsimp simp add: const_def split: if_splits)
 	next case goal5 thus ?case by(clarsimp simp add: const_def split: if_splits)
 	next
 		case goal6
 		from goal6 have s: "Rmi_g ni1 n1 s" "Rmi_g ni2 n2 s" by simp_all
-		have sn: "pointermap_sane s" using goal6(1) by simp
+		have sn: "pointermap_sane s" using goal6(1) unfolding bdd_sane_def by simp
 		note lesI = ifmi_les[OF `pointermap_sane s`  `ifmi v ni1 ni2 s = (ni, s')`]
 		from s goal6(3) have "Rmi_g ni (IFC v n1 n2) s'"
 		proof(cases "ni1 = ni2")
@@ -175,9 +404,10 @@ proof  -
 			apply(clarsimp split: prod.splits)
 		done
 	next
-		case goal12 thus ?case using ifmi_saneI by blast
+		case goal12 
+		thus ?case by(blast dest: bdd_node_valid_RmiI ifmi_saneI2)
 	next
-		case goal13 thus ?case using rmigneq by fastforce
+		case goal13 thus ?case using rmigneq bdd_sane_def by fastforce
 	next
 		case goal14 thus ?case by (simp add: rmigeq)
 	qed(simp_all)
